changes to openid

src/Examples/OpenIDLogin/VProgram/CorralTmpConcatFile.bpl
@@ -2156,9 +2156,17 @@ procedure {:extern} CST.CST_Ops.Certify$CST.CST_Struct(msg$in: Ref) returns ($re
 
 const {:value "UserID"} unique $string_literal_UserID_13: Ref;
 
+procedure {:extern} System.Web.HttpSessionStateBase.get_Item$System.String($this: Ref, name$in: Ref) returns ($result: Ref);
+
+
+
 const {:value ""} unique $string_literal__14: Ref;
 
-procedure {:extern} System.Web.SessionState.HttpSessionState.set_Item$System.String$System.Object($this: Ref, name$in: Ref, value$in: Ref);
+procedure {:extern} System.Web.HttpSessionStateBase.set_Item$System.String$System.Object($this: Ref, name$in: Ref, value$in: Ref);
+
+
+
+procedure {:extern} System.Web.HttpSessionStateBase.Add$System.String$System.Object($this: Ref, name$in: Ref, value$in: Ref);
 
 
 
@@ -2169,6 +2177,10 @@ implementation GenericAuthNameSpace.RP.AuthenticationDone$GenericAuthNameSpace.R
   var $tmp0: bool;
   var $tmp1: Ref;
   var $tmp2: Ref;
+  var $tmp3: Ref;
+  var $tmp4: Ref;
+  var $tmp5: Ref;
+  var $tmp6: Ref;
   var local_1_bool: bool;
   var $localExc: Ref;
   var $label: int;
@@ -2179,20 +2191,44 @@ implementation GenericAuthNameSpace.RP.AuthenticationDone$GenericAuthNameSpace.R
     local_0_bool := $tmp0;
     assume $this != null;
     $tmp1 := F$GenericAuthNameSpace.RP.CurrentSession[$this];
-    if (local_0_bool)
+    call $tmp2 := System.Web.HttpSessionStateBase.get_Item$System.String($tmp1, $string_literal_UserID_13);
+    if ($tmp2 != null)
     {
-        $tmp2 := conclusion;
-        assume $tmp2 != null;
+        assume {:breadcrumb 63} true;
+        assume $this != null;
+        $tmp3 := F$GenericAuthNameSpace.RP.CurrentSession[$this];
+        if (local_0_bool)
+        {
+            $tmp4 := conclusion;
+            assume $tmp4 != null;
+        }
+        else
+        {
+        }
+
+        call System.Web.HttpSessionStateBase.set_Item$System.String$System.Object($tmp3, $string_literal_UserID_13, (if local_0_bool then F$GenericAuthNameSpace.RP.AuthenticationConclusion.SessionUID[$tmp4] else $string_literal__14));
     }
     else
     {
+        assume {:breadcrumb 64} true;
+        assume $this != null;
+        $tmp5 := F$GenericAuthNameSpace.RP.CurrentSession[$this];
+        if (local_0_bool)
+        {
+            $tmp6 := conclusion;
+            assume $tmp6 != null;
+        }
+        else
+        {
+        }
+
+        call System.Web.HttpSessionStateBase.Add$System.String$System.Object($tmp5, $string_literal_UserID_13, (if local_0_bool then F$GenericAuthNameSpace.RP.AuthenticationConclusion.SessionUID[$tmp6] else $string_literal__14));
     }
 
-    call System.Web.SessionState.HttpSessionState.set_Item$System.String$System.Object($tmp1, $string_literal_UserID_13, (if local_0_bool then F$GenericAuthNameSpace.RP.AuthenticationConclusion.SessionUID[$tmp2] else $string_literal__14));
     local_1_bool := local_0_bool;
-    goto IL_002e;
+    goto IL_0069;
 
-  IL_002e:
+  IL_0069:
     $result := local_1_bool;
     return;
 }
@@ -2207,7 +2243,7 @@ implementation GenericAuthNameSpace.RP.#ctor($this: Ref)
     F$GenericAuthNameSpace.RP.CurrentSession[$this] := null;
     F$GenericAuthNameSpace.RP.Domain[$this] := null;
     F$GenericAuthNameSpace.RP.Realm[$this] := null;
-    assume {:breadcrumb 63} true;
+    assume {:breadcrumb 65} true;
     call System.Object.#ctor($this);
 }
 
@@ -2223,7 +2259,7 @@ implementation GenericAuthNameSpace.RP.AuthenticationConclusion.#ctor($this: Ref
   var $label: int;
 
     F$GenericAuthNameSpace.RP.AuthenticationConclusion.SessionUID[$this] := null;
-    assume {:breadcrumb 64} true;
+    assume {:breadcrumb 66} true;
     call CST.CST_Struct.#ctor($this);
 }
 
@@ -2258,7 +2294,7 @@ implementation GenericAuthNameSpace.SignInIdP_Resp_SignInRP_Req.#ctor($this: Ref
   var $localExc: Ref;
   var $label: int;
 
-    assume {:breadcrumb 65} true;
+    assume {:breadcrumb 67} true;
     call CST.CST_Struct.#ctor($this);
 }
 
@@ -2279,7 +2315,7 @@ implementation GenericAuthNameSpace.SignInRP_Resp.#ctor($this: Ref)
   var $localExc: Ref;
   var $label: int;
 
-    assume {:breadcrumb 66} true;
+    assume {:breadcrumb 68} true;
     call CST.CST_Struct.#ctor($this);
 }
 
@@ -2304,7 +2340,7 @@ implementation GenericAuthNameSpace.ID_Claim.#ctor($this: Ref)
   var $localExc: Ref;
   var $label: int;
 
-    assume {:breadcrumb 67} true;
+    assume {:breadcrumb 69} true;
     call System.Object.#ctor($this);
 }
 
@@ -2351,7 +2387,7 @@ implementation GenericAuthNameSpace.GlobalObjects_base.Assert_BadPersonCannotSig
   var $label: int;
 
     conclusion := conclusion$in;
-    assume {:breadcrumb 68} true;
+    assume {:breadcrumb 70} true;
     $tmp10 := F$GenericAuthNameSpace.GlobalObjects_base.IdP;
     assume $tmp10 != null;
     if ($TypeConstructor($DynamicType(F$GenericAuthNameSpace.IdP.IdpAuthRecs[$tmp10])) == T$OpenID20NameSpace.Yahoo_IdP.IDAssertionRecsDictionary_def)
@@ -2419,7 +2455,7 @@ implementation GenericAuthNameSpace.GlobalObjects_base.#ctor($this: Ref)
   var $localExc: Ref;
   var $label: int;
 
-    assume {:breadcrumb 69} true;
+    assume {:breadcrumb 71} true;
     call System.Object.#ctor($this);
 }
 
@@ -2452,7 +2488,7 @@ implementation GenericAuthNameSpace.SignInIdP_Req.#ctor($this: Ref)
   var $label: int;
 
     F$GenericAuthNameSpace.SignInIdP_Req.IdPSessionSecret[$this] := null;
-    assume {:breadcrumb 70} true;
+    assume {:breadcrumb 72} true;
     call CST.CST_Struct.#ctor($this);
 }
 
@@ -2511,16 +2547,16 @@ implementation GenericAuthNameSpace.IdP.SignInIdP$GenericAuthNameSpace.SignInIdP
   var $label: int;
 
     req := req$in;
-    assume {:breadcrumb 71} true;
+    assume {:breadcrumb 73} true;
     F$GenericAuthNameSpace.GlobalObjects_base.SignInIdP_Req := req;
     if (req == null)
     {
-        assume {:breadcrumb 72} true;
+        assume {:breadcrumb 74} true;
         local_1_Ref := null;
     }
     else
     {
-        assume {:breadcrumb 73} true;
+        assume {:breadcrumb 75} true;
         if ($TypeConstructor($DynamicType($this)) == T$OpenID20NameSpace.Yahoo_IdP)
         {
             call $tmp0 := OpenID20NameSpace.OpenIDProvider.Process_SignInIdP_req$GenericAuthNameSpace.SignInIdP_Req($this, req);
@@ -2576,12 +2612,12 @@ implementation GenericAuthNameSpace.IdP.SignInIdP$GenericAuthNameSpace.SignInIdP
 
         if (!(if $TypeConstructor($DynamicType(F$GenericAuthNameSpace.IdP.IdpAuthRecs[$this])) == T$OpenID20NameSpace.Yahoo_IdP.IDAssertionRecsDictionary_def then $tmp7 else $tmp12))
         {
-            assume {:breadcrumb 74} true;
+            assume {:breadcrumb 76} true;
             local_1_Ref := null;
         }
         else
         {
-            assume {:breadcrumb 75} true;
+            assume {:breadcrumb 77} true;
             if ($TypeConstructor($DynamicType($this)) == T$OpenID20NameSpace.Yahoo_IdP)
             {
                 if ($TypeConstructor($DynamicType(local_0_Ref)) == T$OpenID20NameSpace.IDAssertionEntry)
@@ -2643,7 +2679,7 @@ implementation GenericAuthNameSpace.IdP.#ctor($this: Ref)
   var $label: int;
 
     F$GenericAuthNameSpace.IdP.IdpAuthRecs[$this] := null;
-    assume {:breadcrumb 76} true;
+    assume {:breadcrumb 78} true;
     call System.Object.#ctor($this);
 }
 
@@ -2696,6 +2732,16 @@ procedure {:extern} System.Web.UI.Page.get_Request($this: Ref) returns ($result:
 procedure {:extern} System.Web.UI.Page.get_Session($this: Ref) returns ($result: Ref);
 
 
+
+procedure {:extern} System.Web.HttpSessionStateWrapper.#ctor$System.Web.SessionState.HttpSessionState($this: Ref, httpSessionState$in: Ref);
+
+
+
+function {:extern} T$System.Web.HttpSessionStateWrapper() : Ref;
+
+const {:extern} unique T$System.Web.HttpSessionStateWrapper: int;
+
+axiom $TypeConstructor(T$System.Web.HttpSessionStateWrapper()) == T$System.Web.HttpSessionStateWrapper;
 
 procedure {:extern} System.Web.UI.Page.set_Visible$System.Boolean($this: Ref, value$in: bool);
 
@@ -2782,12 +2828,13 @@ implementation OpenIDExample.LogIn.Page_Load$System.Object$System.EventArgs($thi
   var $tmp46: Ref;
   var $tmp47: Ref;
   var $tmp48: Ref;
+  var $tmp49: Ref;
   var $localExc: Ref;
   var $label: int;
 
     sender := sender$in;
     e := e$in;
-    assume {:breadcrumb 77} true;
+    assume {:breadcrumb 79} true;
     call $tmp3 := System.Web.UI.Page.get_Request($this);
     call $tmp4 := System.Web.HttpRequest.get_Params($tmp3);
     call $tmp5 := System.Collections.Specialized.NameValueCollection.get_Item$System.String($tmp4, $string_literal_openid.mode_5);
@@ -2805,31 +2852,35 @@ implementation OpenIDExample.LogIn.Page_Load$System.Object$System.EventArgs($thi
 
     if ((if !$tmp6 then $tmp2 else false))
     {
-        assume {:breadcrumb 78} true;
+        assume {:breadcrumb 80} true;
         if (!F$OpenIDExample.LogIn.expecting_redir)
         {
-            assume {:breadcrumb 80} true;
+            assume {:breadcrumb 82} true;
             return;
         }
         else
         {
-            assume {:breadcrumb 81} true;
+            assume {:breadcrumb 83} true;
         }
 
         F$OpenIDExample.LogIn.expecting_redir := false;
-        call $tmp7 := System.Web.UI.Page.get_Session($this);
+        call $tmp7 := Alloc();
+        call $tmp8 := System.Web.UI.Page.get_Session($this);
+        call System.Web.HttpSessionStateWrapper.#ctor$System.Web.SessionState.HttpSessionState($tmp7, $tmp8);
+        assume $DynamicType($tmp7) == T$System.Web.HttpSessionStateWrapper();
+        assume $TypeConstructor($DynamicType($tmp7)) == T$System.Web.HttpSessionStateWrapper;
         assume $this != null;
         F$GenericAuthNameSpace.RP.CurrentSession[F$OpenIDExample.LogIn.RP[$this]] := $tmp7;
         assume $this != null;
         if ($TypeConstructor($DynamicType(F$OpenIDExample.LogIn.RP[$this])) == T$LiveIDNameSpace.Yahoo_RP_For_vProgram)
         {
             assume $this != null;
-            $tmp8 := F$OpenIDExample.LogIn.RP[$this];
-            assume $this != null;
             $tmp9 := F$OpenIDExample.LogIn.RP[$this];
-            call $tmp10 := System.Web.UI.Page.get_Request($this);
-            call $tmp11 := OpenID20NameSpace.RelyingParty.ParseAuthenticationResponse$System.Web.HttpRequest($tmp9, $tmp10);
-            call $tmp12 := OpenID20NameSpace.RelyingParty.SignInRP$GenericAuthNameSpace.SignInIdP_Resp_SignInRP_Req($tmp8, $tmp11);
+            assume $this != null;
+            $tmp10 := F$OpenIDExample.LogIn.RP[$this];
+            call $tmp11 := System.Web.UI.Page.get_Request($this);
+            call $tmp12 := OpenID20NameSpace.RelyingParty.ParseAuthenticationResponse$System.Web.HttpRequest($tmp10, $tmp11);
+            call $tmp13 := OpenID20NameSpace.RelyingParty.SignInRP$GenericAuthNameSpace.SignInIdP_Resp_SignInRP_Req($tmp9, $tmp12);
         }
         else
         {
@@ -2837,12 +2888,12 @@ implementation OpenIDExample.LogIn.Page_Load$System.Object$System.EventArgs($thi
             if ($TypeConstructor($DynamicType(F$OpenIDExample.LogIn.RP[$this])) == T$OpenID20NameSpace.Yahoo_RP)
             {
                 assume $this != null;
-                $tmp13 := F$OpenIDExample.LogIn.RP[$this];
-                assume $this != null;
                 $tmp14 := F$OpenIDExample.LogIn.RP[$this];
-                call $tmp15 := System.Web.UI.Page.get_Request($this);
-                call $tmp16 := OpenID20NameSpace.RelyingParty.ParseAuthenticationResponse$System.Web.HttpRequest($tmp14, $tmp15);
-                call $tmp17 := OpenID20NameSpace.RelyingParty.SignInRP$GenericAuthNameSpace.SignInIdP_Resp_SignInRP_Req($tmp13, $tmp16);
+                assume $this != null;
+                $tmp15 := F$OpenIDExample.LogIn.RP[$this];
+                call $tmp16 := System.Web.UI.Page.get_Request($this);
+                call $tmp17 := OpenID20NameSpace.RelyingParty.ParseAuthenticationResponse$System.Web.HttpRequest($tmp15, $tmp16);
+                call $tmp18 := OpenID20NameSpace.RelyingParty.SignInRP$GenericAuthNameSpace.SignInIdP_Resp_SignInRP_Req($tmp14, $tmp17);
             }
             else
             {
@@ -2850,22 +2901,22 @@ implementation OpenIDExample.LogIn.Page_Load$System.Object$System.EventArgs($thi
                 if ($TypeConstructor($DynamicType(F$OpenIDExample.LogIn.RP[$this])) == T$OpenID20NameSpace.RelyingParty)
                 {
                     assume $this != null;
-                    $tmp18 := F$OpenIDExample.LogIn.RP[$this];
-                    assume $this != null;
                     $tmp19 := F$OpenIDExample.LogIn.RP[$this];
-                    call $tmp20 := System.Web.UI.Page.get_Request($this);
-                    call $tmp21 := OpenID20NameSpace.RelyingParty.ParseAuthenticationResponse$System.Web.HttpRequest($tmp19, $tmp20);
-                    call $tmp22 := OpenID20NameSpace.RelyingParty.SignInRP$GenericAuthNameSpace.SignInIdP_Resp_SignInRP_Req($tmp18, $tmp21);
+                    assume $this != null;
+                    $tmp20 := F$OpenIDExample.LogIn.RP[$this];
+                    call $tmp21 := System.Web.UI.Page.get_Request($this);
+                    call $tmp22 := OpenID20NameSpace.RelyingParty.ParseAuthenticationResponse$System.Web.HttpRequest($tmp20, $tmp21);
+                    call $tmp23 := OpenID20NameSpace.RelyingParty.SignInRP$GenericAuthNameSpace.SignInIdP_Resp_SignInRP_Req($tmp19, $tmp22);
                 }
                 else
                 {
                     assume $this != null;
-                    $tmp23 := F$OpenIDExample.LogIn.RP[$this];
-                    assume $this != null;
                     $tmp24 := F$OpenIDExample.LogIn.RP[$this];
-                    call $tmp25 := System.Web.UI.Page.get_Request($this);
-                    call $tmp26 := OpenID20NameSpace.RelyingParty.ParseAuthenticationResponse$System.Web.HttpRequest($tmp24, $tmp25);
-                    call $tmp27 := GenericAuthNameSpace.RP.SignInRP$GenericAuthNameSpace.SignInIdP_Resp_SignInRP_Req($tmp23, $tmp26);
+                    assume $this != null;
+                    $tmp25 := F$OpenIDExample.LogIn.RP[$this];
+                    call $tmp26 := System.Web.UI.Page.get_Request($this);
+                    call $tmp27 := OpenID20NameSpace.RelyingParty.ParseAuthenticationResponse$System.Web.HttpRequest($tmp25, $tmp26);
+                    call $tmp28 := GenericAuthNameSpace.RP.SignInRP$GenericAuthNameSpace.SignInIdP_Resp_SignInRP_Req($tmp24, $tmp27);
                 }
             }
         }
@@ -2873,39 +2924,39 @@ implementation OpenIDExample.LogIn.Page_Load$System.Object$System.EventArgs($thi
         assume $this != null;
         if ($TypeConstructor($DynamicType(F$OpenIDExample.LogIn.notLoggedIn[$this])) == T$OpenIDExample.LogIn)
         {
-            assume {:breadcrumb 82} true;
+            assume {:breadcrumb 84} true;
             assume $this != null;
-            $tmp28 := F$OpenIDExample.LogIn.notLoggedIn[$this];
-            call System.Web.UI.Page.set_Visible$System.Boolean($tmp28, false);
+            $tmp29 := F$OpenIDExample.LogIn.notLoggedIn[$this];
+            call System.Web.UI.Page.set_Visible$System.Boolean($tmp29, false);
         }
         else
         {
-            assume {:breadcrumb 83} true;
+            assume {:breadcrumb 85} true;
             assume $this != null;
             if ($TypeConstructor($DynamicType(F$OpenIDExample.LogIn.notLoggedIn[$this])) == T$System.Web.UI.Page)
             {
-                assume {:breadcrumb 84} true;
+                assume {:breadcrumb 86} true;
                 assume $this != null;
-                $tmp29 := F$OpenIDExample.LogIn.notLoggedIn[$this];
-                call System.Web.UI.Page.set_Visible$System.Boolean($tmp29, false);
+                $tmp30 := F$OpenIDExample.LogIn.notLoggedIn[$this];
+                call System.Web.UI.Page.set_Visible$System.Boolean($tmp30, false);
             }
             else
             {
-                assume {:breadcrumb 85} true;
+                assume {:breadcrumb 87} true;
                 assume $this != null;
                 if ($TypeConstructor($DynamicType(F$OpenIDExample.LogIn.notLoggedIn[$this])) == T$System.Web.UI.TemplateControl)
                 {
-                    assume {:breadcrumb 86} true;
-                    assume $this != null;
-                    $tmp30 := F$OpenIDExample.LogIn.notLoggedIn[$this];
-                    call System.Web.UI.Control.set_Visible$System.Boolean($tmp30, false);
-                }
-                else
-                {
-                    assume {:breadcrumb 87} true;
+                    assume {:breadcrumb 88} true;
                     assume $this != null;
                     $tmp31 := F$OpenIDExample.LogIn.notLoggedIn[$this];
                     call System.Web.UI.Control.set_Visible$System.Boolean($tmp31, false);
+                }
+                else
+                {
+                    assume {:breadcrumb 89} true;
+                    assume $this != null;
+                    $tmp32 := F$OpenIDExample.LogIn.notLoggedIn[$this];
+                    call System.Web.UI.Control.set_Visible$System.Boolean($tmp32, false);
                 }
             }
         }
@@ -2913,93 +2964,93 @@ implementation OpenIDExample.LogIn.Page_Load$System.Object$System.EventArgs($thi
         assume $this != null;
         if ($TypeConstructor($DynamicType(F$OpenIDExample.LogIn.LoggedIn[$this])) == T$OpenIDExample.LogIn)
         {
-            assume {:breadcrumb 88} true;
+            assume {:breadcrumb 90} true;
             assume $this != null;
-            $tmp32 := F$OpenIDExample.LogIn.LoggedIn[$this];
-            call System.Web.UI.Page.set_Visible$System.Boolean($tmp32, true);
+            $tmp33 := F$OpenIDExample.LogIn.LoggedIn[$this];
+            call System.Web.UI.Page.set_Visible$System.Boolean($tmp33, true);
         }
         else
         {
-            assume {:breadcrumb 89} true;
+            assume {:breadcrumb 91} true;
             assume $this != null;
             if ($TypeConstructor($DynamicType(F$OpenIDExample.LogIn.LoggedIn[$this])) == T$System.Web.UI.Page)
             {
-                assume {:breadcrumb 90} true;
+                assume {:breadcrumb 92} true;
                 assume $this != null;
-                $tmp33 := F$OpenIDExample.LogIn.LoggedIn[$this];
-                call System.Web.UI.Page.set_Visible$System.Boolean($tmp33, true);
+                $tmp34 := F$OpenIDExample.LogIn.LoggedIn[$this];
+                call System.Web.UI.Page.set_Visible$System.Boolean($tmp34, true);
             }
             else
             {
-                assume {:breadcrumb 91} true;
+                assume {:breadcrumb 93} true;
                 assume $this != null;
                 if ($TypeConstructor($DynamicType(F$OpenIDExample.LogIn.LoggedIn[$this])) == T$System.Web.UI.TemplateControl)
                 {
-                    assume {:breadcrumb 92} true;
-                    assume $this != null;
-                    $tmp34 := F$OpenIDExample.LogIn.LoggedIn[$this];
-                    call System.Web.UI.Control.set_Visible$System.Boolean($tmp34, true);
-                }
-                else
-                {
-                    assume {:breadcrumb 93} true;
+                    assume {:breadcrumb 94} true;
                     assume $this != null;
                     $tmp35 := F$OpenIDExample.LogIn.LoggedIn[$this];
                     call System.Web.UI.Control.set_Visible$System.Boolean($tmp35, true);
+                }
+                else
+                {
+                    assume {:breadcrumb 95} true;
+                    assume $this != null;
+                    $tmp36 := F$OpenIDExample.LogIn.LoggedIn[$this];
+                    call System.Web.UI.Control.set_Visible$System.Boolean($tmp36, true);
                 }
             }
         }
 
         assume $this != null;
-        $tmp36 := F$OpenIDExample.LogIn.logged_id[$this];
-        call $tmp37 := System.Web.UI.Page.get_Request($this);
-        call $tmp38 := System.Web.HttpRequest.get_Params($tmp37);
-        call $tmp39 := System.Collections.Specialized.NameValueCollection.get_Item$System.String($tmp38, $string_literal_openid.identity_16);
-        call $tmp40 := System.String.Format$System.String$System.Object($string_literal_Your$ID$is$$0$_15, $tmp39);
-        call System.Web.UI.HtmlControls.HtmlContainerControl.set_InnerHtml$System.String($tmp36, $tmp40);
+        $tmp37 := F$OpenIDExample.LogIn.logged_id[$this];
+        call $tmp38 := System.Web.UI.Page.get_Request($this);
+        call $tmp39 := System.Web.HttpRequest.get_Params($tmp38);
+        call $tmp40 := System.Collections.Specialized.NameValueCollection.get_Item$System.String($tmp39, $string_literal_openid.identity_16);
+        call $tmp41 := System.String.Format$System.String$System.Object($string_literal_Your$ID$is$$0$_15, $tmp40);
+        call System.Web.UI.HtmlControls.HtmlContainerControl.set_InnerHtml$System.String($tmp37, $tmp41);
         return;
     }
     else
     {
-        assume {:breadcrumb 79} true;
+        assume {:breadcrumb 81} true;
     }
 
     assume $this != null;
     if ($TypeConstructor($DynamicType(F$OpenIDExample.LogIn.notLoggedIn[$this])) == T$OpenIDExample.LogIn)
     {
-        assume {:breadcrumb 94} true;
+        assume {:breadcrumb 96} true;
         assume $this != null;
-        $tmp41 := F$OpenIDExample.LogIn.notLoggedIn[$this];
-        call System.Web.UI.Page.set_Visible$System.Boolean($tmp41, true);
+        $tmp42 := F$OpenIDExample.LogIn.notLoggedIn[$this];
+        call System.Web.UI.Page.set_Visible$System.Boolean($tmp42, true);
     }
     else
     {
-        assume {:breadcrumb 95} true;
+        assume {:breadcrumb 97} true;
         assume $this != null;
         if ($TypeConstructor($DynamicType(F$OpenIDExample.LogIn.notLoggedIn[$this])) == T$System.Web.UI.Page)
         {
-            assume {:breadcrumb 96} true;
+            assume {:breadcrumb 98} true;
             assume $this != null;
-            $tmp42 := F$OpenIDExample.LogIn.notLoggedIn[$this];
-            call System.Web.UI.Page.set_Visible$System.Boolean($tmp42, true);
+            $tmp43 := F$OpenIDExample.LogIn.notLoggedIn[$this];
+            call System.Web.UI.Page.set_Visible$System.Boolean($tmp43, true);
         }
         else
         {
-            assume {:breadcrumb 97} true;
+            assume {:breadcrumb 99} true;
             assume $this != null;
             if ($TypeConstructor($DynamicType(F$OpenIDExample.LogIn.notLoggedIn[$this])) == T$System.Web.UI.TemplateControl)
             {
-                assume {:breadcrumb 98} true;
-                assume $this != null;
-                $tmp43 := F$OpenIDExample.LogIn.notLoggedIn[$this];
-                call System.Web.UI.Control.set_Visible$System.Boolean($tmp43, true);
-            }
-            else
-            {
-                assume {:breadcrumb 99} true;
+                assume {:breadcrumb 100} true;
                 assume $this != null;
                 $tmp44 := F$OpenIDExample.LogIn.notLoggedIn[$this];
                 call System.Web.UI.Control.set_Visible$System.Boolean($tmp44, true);
+            }
+            else
+            {
+                assume {:breadcrumb 101} true;
+                assume $this != null;
+                $tmp45 := F$OpenIDExample.LogIn.notLoggedIn[$this];
+                call System.Web.UI.Control.set_Visible$System.Boolean($tmp45, true);
             }
         }
     }
@@ -3007,39 +3058,39 @@ implementation OpenIDExample.LogIn.Page_Load$System.Object$System.EventArgs($thi
     assume $this != null;
     if ($TypeConstructor($DynamicType(F$OpenIDExample.LogIn.LoggedIn[$this])) == T$OpenIDExample.LogIn)
     {
-        assume {:breadcrumb 100} true;
+        assume {:breadcrumb 102} true;
         assume $this != null;
-        $tmp45 := F$OpenIDExample.LogIn.LoggedIn[$this];
-        call System.Web.UI.Page.set_Visible$System.Boolean($tmp45, false);
+        $tmp46 := F$OpenIDExample.LogIn.LoggedIn[$this];
+        call System.Web.UI.Page.set_Visible$System.Boolean($tmp46, false);
     }
     else
     {
-        assume {:breadcrumb 101} true;
+        assume {:breadcrumb 103} true;
         assume $this != null;
         if ($TypeConstructor($DynamicType(F$OpenIDExample.LogIn.LoggedIn[$this])) == T$System.Web.UI.Page)
         {
-            assume {:breadcrumb 102} true;
+            assume {:breadcrumb 104} true;
             assume $this != null;
-            $tmp46 := F$OpenIDExample.LogIn.LoggedIn[$this];
-            call System.Web.UI.Page.set_Visible$System.Boolean($tmp46, false);
+            $tmp47 := F$OpenIDExample.LogIn.LoggedIn[$this];
+            call System.Web.UI.Page.set_Visible$System.Boolean($tmp47, false);
         }
         else
         {
-            assume {:breadcrumb 103} true;
+            assume {:breadcrumb 105} true;
             assume $this != null;
             if ($TypeConstructor($DynamicType(F$OpenIDExample.LogIn.LoggedIn[$this])) == T$System.Web.UI.TemplateControl)
             {
-                assume {:breadcrumb 104} true;
-                assume $this != null;
-                $tmp47 := F$OpenIDExample.LogIn.LoggedIn[$this];
-                call System.Web.UI.Control.set_Visible$System.Boolean($tmp47, false);
-            }
-            else
-            {
-                assume {:breadcrumb 105} true;
+                assume {:breadcrumb 106} true;
                 assume $this != null;
                 $tmp48 := F$OpenIDExample.LogIn.LoggedIn[$this];
                 call System.Web.UI.Control.set_Visible$System.Boolean($tmp48, false);
+            }
+            else
+            {
+                assume {:breadcrumb 107} true;
+                assume $this != null;
+                $tmp49 := F$OpenIDExample.LogIn.LoggedIn[$this];
+                call System.Web.UI.Control.set_Visible$System.Boolean($tmp49, false);
             }
         }
     }
@@ -3103,7 +3154,7 @@ implementation OpenIDExample.LogIn.LoginBtn_Click$System.Object$System.EventArgs
 
     sender := sender$in;
     e := e$in;
-    assume {:breadcrumb 106} true;
+    assume {:breadcrumb 108} true;
     F$OpenIDExample.LogIn.expecting_redir := true;
     assume $this != null;
     $tmp0 := F$OpenIDExample.LogIn.RP[$this];
@@ -3174,40 +3225,40 @@ implementation OpenIDExample.LogIn.LogoutBtn_Click$System.Object$System.EventArg
 
     sender := sender$in;
     e := e$in;
-    assume {:breadcrumb 107} true;
+    assume {:breadcrumb 109} true;
     assume $this != null;
     if ($TypeConstructor($DynamicType(F$OpenIDExample.LogIn.notLoggedIn[$this])) == T$OpenIDExample.LogIn)
     {
-        assume {:breadcrumb 108} true;
+        assume {:breadcrumb 110} true;
         assume $this != null;
         $tmp0 := F$OpenIDExample.LogIn.notLoggedIn[$this];
         call System.Web.UI.Page.set_Visible$System.Boolean($tmp0, true);
     }
     else
     {
-        assume {:breadcrumb 109} true;
+        assume {:breadcrumb 111} true;
         assume $this != null;
         if ($TypeConstructor($DynamicType(F$OpenIDExample.LogIn.notLoggedIn[$this])) == T$System.Web.UI.Page)
         {
-            assume {:breadcrumb 110} true;
+            assume {:breadcrumb 112} true;
             assume $this != null;
             $tmp1 := F$OpenIDExample.LogIn.notLoggedIn[$this];
             call System.Web.UI.Page.set_Visible$System.Boolean($tmp1, true);
         }
         else
         {
-            assume {:breadcrumb 111} true;
+            assume {:breadcrumb 113} true;
             assume $this != null;
             if ($TypeConstructor($DynamicType(F$OpenIDExample.LogIn.notLoggedIn[$this])) == T$System.Web.UI.TemplateControl)
             {
-                assume {:breadcrumb 112} true;
+                assume {:breadcrumb 114} true;
                 assume $this != null;
                 $tmp2 := F$OpenIDExample.LogIn.notLoggedIn[$this];
                 call System.Web.UI.Control.set_Visible$System.Boolean($tmp2, true);
             }
             else
             {
-                assume {:breadcrumb 113} true;
+                assume {:breadcrumb 115} true;
                 assume $this != null;
                 $tmp3 := F$OpenIDExample.LogIn.notLoggedIn[$this];
                 call System.Web.UI.Control.set_Visible$System.Boolean($tmp3, true);
@@ -3218,36 +3269,36 @@ implementation OpenIDExample.LogIn.LogoutBtn_Click$System.Object$System.EventArg
     assume $this != null;
     if ($TypeConstructor($DynamicType(F$OpenIDExample.LogIn.LoggedIn[$this])) == T$OpenIDExample.LogIn)
     {
-        assume {:breadcrumb 114} true;
+        assume {:breadcrumb 116} true;
         assume $this != null;
         $tmp4 := F$OpenIDExample.LogIn.LoggedIn[$this];
         call System.Web.UI.Page.set_Visible$System.Boolean($tmp4, false);
     }
     else
     {
-        assume {:breadcrumb 115} true;
+        assume {:breadcrumb 117} true;
         assume $this != null;
         if ($TypeConstructor($DynamicType(F$OpenIDExample.LogIn.LoggedIn[$this])) == T$System.Web.UI.Page)
         {
-            assume {:breadcrumb 116} true;
+            assume {:breadcrumb 118} true;
             assume $this != null;
             $tmp5 := F$OpenIDExample.LogIn.LoggedIn[$this];
             call System.Web.UI.Page.set_Visible$System.Boolean($tmp5, false);
         }
         else
         {
-            assume {:breadcrumb 117} true;
+            assume {:breadcrumb 119} true;
             assume $this != null;
             if ($TypeConstructor($DynamicType(F$OpenIDExample.LogIn.LoggedIn[$this])) == T$System.Web.UI.TemplateControl)
             {
-                assume {:breadcrumb 118} true;
+                assume {:breadcrumb 120} true;
                 assume $this != null;
                 $tmp6 := F$OpenIDExample.LogIn.LoggedIn[$this];
                 call System.Web.UI.Control.set_Visible$System.Boolean($tmp6, false);
             }
             else
             {
-                assume {:breadcrumb 119} true;
+                assume {:breadcrumb 121} true;
                 assume $this != null;
                 $tmp7 := F$OpenIDExample.LogIn.LoggedIn[$this];
                 call System.Web.UI.Control.set_Visible$System.Boolean($tmp7, false);
@@ -3285,7 +3336,7 @@ implementation OpenIDExample.LogIn.#ctor($this: Ref)
     F$OpenIDExample.LogIn.LoggedIn[$this] := null;
     F$OpenIDExample.LogIn.logged_id[$this] := null;
     F$OpenIDExample.LogIn.Logout[$this] := null;
-    assume {:breadcrumb 120} true;
+    assume {:breadcrumb 122} true;
     call $tmp0 := Alloc();
     call OpenID20NameSpace.Yahoo_RP.#ctor$System.String$System.String($tmp0, $string_literal_http$$$localhost$32928$LogIn.aspx_19, F$OpenIDExample.LogIn.yahoo_str);
     assume $DynamicType($tmp0) == T$OpenID20NameSpace.Yahoo_RP();
@@ -3309,7 +3360,7 @@ implementation OpenIDExample.LogIn.#cctor()
 
     F$OpenIDExample.LogIn.yahoo_str := null;
     F$OpenIDExample.LogIn.expecting_redir := false;
-    assume {:breadcrumb 121} true;
+    assume {:breadcrumb 123} true;
     F$OpenIDExample.LogIn.yahoo_str := $string_literal_https$$$open.login.yahooapis.com$openid$op$auth_20;
     F$OpenIDExample.LogIn.expecting_redir := false;
 }
@@ -3321,7 +3372,7 @@ implementation OpenID20NameSpace.Yahoo_RP.#ctor($this: Ref)
   var $localExc: Ref;
   var $label: int;
 
-    assume {:breadcrumb 122} true;
+    assume {:breadcrumb 124} true;
     call OpenID20NameSpace.RelyingParty.#ctor($this);
 }
 
@@ -3336,7 +3387,7 @@ implementation OpenID20NameSpace.Yahoo_RP.#ctor$System.String$System.String($thi
 
     return_uri := return_uri$in;
     endpointUrl := endpointUrl$in;
-    assume {:breadcrumb 123} true;
+    assume {:breadcrumb 125} true;
     call OpenID20NameSpace.RelyingParty.#ctor($this);
     call OpenID20NameSpace.RelyingParty.set_return_uri$System.String($this, return_uri);
     F$OpenID20NameSpace.RelyingParty.endpointUrl[$this] := endpointUrl;
@@ -3367,7 +3418,7 @@ implementation OpenID20NameSpace.Yahoo_RP.GenerateURL$OpenID20NameSpace.Authenti
   var $label: int;
 
     req := req$in;
-    assume {:breadcrumb 124} true;
+    assume {:breadcrumb 126} true;
     call $tmp0 := Alloc();
     assume $this != null;
     call System.Text.StringBuilder.#ctor$System.String($tmp0, F$OpenID20NameSpace.RelyingParty.endpointUrl[$this]);
@@ -3405,7 +3456,7 @@ implementation OpenID20NameSpace.Yahoo_RP.GenerateURL$OpenID20NameSpace.Authenti
   var $label: int;
 
     req := req$in;
-    assume {:breadcrumb 125} true;
+    assume {:breadcrumb 127} true;
     call $tmp0 := Alloc();
     assume $this != null;
     call System.Text.StringBuilder.#ctor$System.String($tmp0, F$OpenID20NameSpace.RelyingParty.endpointUrl[$this]);
@@ -3449,7 +3500,7 @@ implementation CST.Debug.reached()
   var $localExc: Ref;
   var $label: int;
 
-    assume {:breadcrumb 126} true;
+    assume {:breadcrumb 128} true;
     assert false;
 }
 
@@ -3464,7 +3515,7 @@ implementation CST.Debug.#ctor($this: Ref)
   var $localExc: Ref;
   var $label: int;
 
-    assume {:breadcrumb 127} true;
+    assume {:breadcrumb 129} true;
     call System.Object.#ctor($this);
 }
 
@@ -3493,7 +3544,7 @@ implementation CST.CST_Struct.#ctor($this: Ref)
 
     F$CST.CST_Struct.SymT[$this] := null;
     F$CST.CST_Struct.SignedBy[$this] := null;
-    assume {:breadcrumb 128} true;
+    assume {:breadcrumb 130} true;
     F$CST.CST_Struct.SymT[$this] := $string_literal__14;
     F$CST.CST_Struct.SignedBy[$this] := $string_literal__14;
     call System.Object.#ctor($this);
@@ -3558,7 +3609,7 @@ implementation OpenID20NameSpace.Yahoo_IdP.init($this: Ref)
   var $localExc: Ref;
   var $label: int;
 
-    assume {:breadcrumb 129} true;
+    assume {:breadcrumb 131} true;
     assume $this != null;
     call OpenID20NameSpace.OpenIDProvider.init$OpenID20NameSpace.IDAssertionRecs($this, F$OpenID20NameSpace.Yahoo_IdP.IDAssertionRecsDictionary[$this]);
     assume $this != null;
@@ -3589,7 +3640,7 @@ implementation OpenID20NameSpace.Yahoo_IdP.#ctor($this: Ref)
   var $label: int;
 
     F$OpenID20NameSpace.Yahoo_IdP.IDAssertionRecsDictionary[$this] := null;
-    assume {:breadcrumb 130} true;
+    assume {:breadcrumb 132} true;
     call $tmp0 := Alloc();
     call OpenID20NameSpace.Yahoo_IdP.IDAssertionRecsDictionary_def.#ctor($tmp0);
     assume $DynamicType($tmp0) == T$OpenID20NameSpace.Yahoo_IdP.IDAssertionRecsDictionary_def();
@@ -3620,7 +3671,7 @@ implementation OpenID20NameSpace.Yahoo_IdP.IDAssertionRecsDictionary_def.getEntr
 
     IdPSessionSecret := IdPSessionSecret$in;
     client_id := client_id$in;
-    assume {:breadcrumb 131} true;
+    assume {:breadcrumb 133} true;
     assume $this != null;
     $tmp0 := F$OpenID20NameSpace.Yahoo_IdP.IDAssertionRecsDictionary_def.Dictionary[$this];
     call $tmp2 := System.Collections.Generic.Dictionary`2.get_Item$`0($tmp0, IdPSessionSecret);
@@ -3656,7 +3707,7 @@ implementation OpenID20NameSpace.Yahoo_IdP.IDAssertionRecsDictionary_def.setEntr
     IdPSessionSecret := IdPSessionSecret$in;
     client_id := client_id$in;
     Entry := Entry$in;
-    assume {:breadcrumb 132} true;
+    assume {:breadcrumb 134} true;
     call $tmp0 := Alloc();
     call OpenID20NameSpace.IDAssertionEntry.#ctor($tmp0);
     assume $DynamicType($tmp0) == T$OpenID20NameSpace.IDAssertionEntry();
@@ -3688,7 +3739,7 @@ implementation OpenID20NameSpace.Yahoo_IdP.IDAssertionRecsDictionary_def.#ctor($
   var $label: int;
 
     F$OpenID20NameSpace.Yahoo_IdP.IDAssertionRecsDictionary_def.Dictionary[$this] := null;
-    assume {:breadcrumb 133} true;
+    assume {:breadcrumb 135} true;
     call $tmp0 := Alloc();
     call System.Collections.Generic.Dictionary`2.#ctor($tmp0);
     assume $DynamicType($tmp0) == T$System.Collections.Generic.Dictionary`2(T$System.String(), T$System.Collections.Generic.Dictionary`2(T$System.String(), T$OpenID20NameSpace.IDAssertionEntry()));
